WIP: LessThan

src/circomlib/bitify.v
@@ -4,6 +4,7 @@ Require Import Coq.Arith.PeanoNat.
 Require Import Coq.Arith.Compare_dec.
 Require Import Coq.PArith.BinPosDef.
 Require Import Coq.ZArith.Znumtheory.
+Require Import Coq.NArith.Nnat.
 
 Require Import Crypto.Spec.ModularArithmetic.
 Require Import Crypto.Spec.ModularArithmetic.
@@ -24,8 +25,12 @@ Require Import Util.
 * https://github.com/iden3/circomlib/blob/master/circuits/bitify.circom
 *)
 
+
+Section _bitify.
+
 Local Open Scope list_scope.
 Local Open Scope F_scope.
+
 
 Context (q:positive) {prime_q:prime q}.
 
@@ -36,15 +41,135 @@ Context (q:positive) {prime_q:prime q}.
 
 Definition F_q := F q.
 
+Locate of_nat.
+
+Lemma length_nil {A: Type} : length (@nil A) = Nat.zero.
+Proof. auto. Qed.
+
+Lemma length_cons_end {A: Type} {n: nat} (w: A) (ws: list A ) (H_ws: length ws = n):
+  length (app ws (w::nil)) = S n.
+Proof.
+  rewrite app_length. simpl. lia.
+Qed.
+
+Lemma length_cons (n: nat) {A: Type}  {ws} {ws'} {w: A} {_: ws' = w :: ws} (H_ws: length ws = n):
+  length ws' = S n.
+Proof. rewrite H. simpl. auto. Qed.
+
 Definition binary (x: F_q) := x = 0 \/ x = 1.
+Definition two : F_q := 1 + 1.
 
-(* WIP: decode a binary signal vector to its value
-Definition decode0b (xs: tuple F n) := fold_right add zero xs.
+(* Aborted approach: Inductive prop (types get too complicated) *)
+(* ws is a big-endian, length-n binary representation of x *)
+(* Inductive repr_binary: forall (x: F q) (n: nat) (ws: list (F q)) (_: length ws = n), Prop :=
+  | repr_binary_nil:
+    repr_binary 0 0%nat nil eq_refl
+  | repr_binary_cons:
+    forall w x n ws H_ws y n' ws' (H_ws': length ws' = n'),
+    binary w -> repr_binary x n ws H_ws ->
+    y = x + w * F.pow two (BinNatDef.N.of_nat n) ->
+    n' = S n ->
+    ws' = w::ws ->
+    repr_binary y n' ws' H_ws'. 
+Lemma repr_binary_test (H: length (1::nil) = 1%nat): repr_binary 1 1%nat (1::nil) H.
+Proof.
+  eapply repr_binary_cons with (w := 1).
+  right. reflexivity.
+  eapply repr_binary_nil.
+  - simpl. replace (two^N0) with (1:F_q). Field.fsatz.
+  admit.
+Admitted.
+*)
 
-Definition w (i: F) := F.pow 2 i.
+Fixpoint repr_to_num (ws: list (F q)) (i: nat) : F q :=
+  match ws with
+  | nil => 0
+  | w::ws' => w * two^(BinNat.N.of_nat i) + repr_to_num ws' (S i)
+  end.
 
-Definition decode_0b_list (xs: list F) :=  
-  *)
+Definition repr_binary x n ws :=
+  length ws = n /\
+  (forall i, i < n -> binary (nth i ws 0)) /\
+  x = repr_to_num ws 0%nat.
+
+Lemma repr_binary_base: repr_binary 0 0%nat nil.
+Proof. unfold repr_binary.
+  split; split.
+  - intros. simpl. destruct i; unfold binary; auto.
+  - reflexivity.
+Qed.
+
+Lemma repr_to_num_S: forall ws i,
+  repr_to_num ws (S i) = two * repr_to_num ws i.
+Proof.
+(* idea: should be a straight forward inductio *)
+Admitted.
+
+
+(* 
+  Lemma repr_binary_ind: forall x n ws w,
+  repr_binary x n ws ->
+  binary w ->
+  repr_binary (x + w * two^(BinNatDef.N.of_nat n)) (S n) (w::ws).
+Proof.
+  unfold repr_binary; intros; split; try split; destruct H; destruct H1.
+  - simpl. auto.
+  - intros.
+    destruct i.
+    + simpl. auto.
+    + simpl. apply H1. lia.
+  - simpl. *)
+
+Definition lt (x y: F_q) := F.to_nat x <= F.to_nat y.
+Definition lt_n (x: F_q) y := F.to_nat x < y.
+Definition geq_n (x: F_q) y := F.to_nat x >= y.
+
+Lemma repr_to_num_trivial: forall ws,
+  (forall i, i < length ws -> binary (nth i ws 0)) ->
+  repr_binary (repr_to_num ws 0) (length ws) ws.
+Proof.
+  induction ws; unfold repr_binary; split; try split; intros; auto.
+Qed.
+
+Theorem repr_binary_ub: forall ws x n,
+  repr_binary x n ws ->
+  lt_n x (2^n)%nat.
+Proof.
+  induction ws. 
+  - unfold repr_binary; intros; simpl in *; destruct H; destruct H0. 
+    subst. cbv. lia.
+  - intros. destruct n; destruct H; destruct H0; simpl in H. lia.
+    inversion H. subst.
+    simpl.
+    assert (H_a: binary a) by (apply (H0 0%nat); lia).
+    destruct H_a; subst.
+    + replace (0 * two ^ N0 + repr_to_num ws 1%nat) with (repr_to_num ws 1%nat) by Field.fsatz.
+      replace (repr_to_num ws 1) with (two * (repr_to_num ws 0%nat)) by (rewrite repr_to_num_S; reflexivity).
+      unfold lt_n.
+      (* Need range check *)
+      replace (F.to_nat (two * repr_to_num ws 0%nat)) with (Nat.add (F.to_nat (repr_to_num ws 0%nat)) (F.to_nat (repr_to_num ws 0%nat)))
+        by admit.
+      simpl.
+      assert (F.to_nat (repr_to_num ws 0%nat) < 2 ^ length ws). {
+        apply IHws.
+        apply repr_to_num_trivial.
+        intros.
+        specialize (H0 (S i)).
+        apply H0. lia.
+      }
+      lia.
+    + (* w = 1 *)
+    admit.
+Admitted.
+
+
+(* If the MSB of ws is 1, then x >= 2^n *)
+Theorem repr_binary_lb: forall x n ws,
+  repr_binary x (S n) ws ->
+  nth 0%nat ws 0 = 1 -> 
+  geq_n x (2^n)%nat.
+Proof.
+Admitted.
 
 
 Definition Num2Bits n (_in: F_q) (_out: tuple F_q n) : Prop :=
@@ -61,34 +186,25 @@ Definition Num2Bits n (_in: F_q) (_out: tuple F_q n) : Prop :=
 
 Theorem Num2Bits_correct n _in _out:
   Num2Bits n _in _out -> (forall i, Nat.lt i n -> binary (Tuple.nth_default 0 i _out)).
-Proof using Type*.
-  pose proof prime_q.
-  pose (Inv := fun i '((lc1, e2, _C): (F.F q * F.F q * Prop)) =>
-    (* match acc with *)
-    (* |  => *)
-      (_C -> (forall j, Nat.lt j i -> binary (Tuple.nth_default 0 j _out)))).
-  pose proof (iter_inv Inv) as Hinv.
+Proof.
   unfold Num2Bits.
-  intros prog i H_i_lt_n.
+  (* provide loop invariant *)
+  pose (Inv := fun i '((lc1, e2, _C): (F.F q * F.F q * Prop)) =>
+    (_C -> (forall j, Nat.lt j i -> binary (Tuple.nth_default 0 j _out)))).
   (* iter initialization *)
   remember (0, 1, True) as a0.
+  intros prog i H_i_lt_n.
   (* iter function *)
   match goal with
   | [ H: context[match ?it ?n ?f ?init with _ => _ end] |- _ ] =>
     let x := fresh "f" in remember f as x
   end.
-  (* Prove Inv hold for initialization *)
-  assert (Hinit: Inv Nat.zero a0).
-  {
-    unfold Inv.
-    rewrite Heqa0. intros _ j impossible.
-    inversion impossible.
-  }
-  (* Prove Inv is inductive *)
-  assert (Hind: forall (j : nat) (b : F.F q * F.F q * Prop),
-    Inv j b -> Inv (S j) (f j b)).
-  {
-    unfold Inv.
+  (* invariant holds *)
+  assert (Hinv: forall i, Inv i (iter i f a0)). {
+  intros. apply iter_inv; unfold Inv.
+  - (* base case *) 
+    subst. intros _ j impossible. lia.
+  - (* inductive case *)
     intros j res Hprev.
     destruct res. destruct p.
     rewrite Heqf.
@@ -97,19 +213,22 @@ Proof using Type*.
     specialize  (Hprev HP).
     assert (H_j0_leq: Nat.le j0 j) by lia.
     destruct (lt_dec j0 j).
-    - auto.
-    - unfold binary.
+    + auto.
+    + unfold binary.
       replace j0 with j by lia.
       destruct (dec (Tuple.nth_default 0 j _out = 0)).
-      + auto.
-      + right.
+      * auto.
+      * right.
+      (* ideally we should use some version of [fsatz], but rn the proof wouldn't type check *)
       rewrite <- Ring.sub_zero_iff.
       apply Hierarchy.zero_product_zero_factor in Hstep.
       destruct (dec (nth_default 0 j _out = 0)); intuition.
   }
-  specialize (Hinv f a0 Hinit Hind n). clear Hind Hinit.
   unfold Inv in Hinv.
+  specialize (Hinv n).
   destruct (iter n f a0).
   destruct p.
   intuition.
 Qed.
+
+End _bitify.
